src/util/data/minimum/default.lean
@@ -1,2 +1,4 @@
 
-import util.data.minimum.basic util.data.minimum.nat util.data.minimum.fin
+import util.data.minimum.basic
+       util.data.minimum.nat util.data.minimum.fin
+       util.data.minimum.lemmas
