src/util/data/minimum/lemmas.lean
@@ -1,0 +1,18 @@
+
+import util.meta.tactic
+
+import util.data.minimum.basic
+
+variable {α : Type*}
+variable [has_minimum α]
+open has_minimum (minimum)
+lemma lt_minimum_iff (x : α) {xs : set α}
+  (h : xs ≠ ∅)
+: x < minimum xs ↔ (∀ y ∈ xs, x < y) :=
+begin
+  split,
+  { intros, apply lt_of_lt_of_le a,
+    apply minimum_le H, },
+  { intros, xassumption,
+    apply minimum_mem h },
+end
