src/util/predicate/basic.lean
@@ -1,0 +1,156 @@
+
+import util.logic
+import util.data.fin
+import util.category
+import util.meta.tactic.basic
+import util.meta.tactic.monotonicity
+
+run_cmd mk_simp_attr `predicate
+
+namespace predicate
+
+universe variables u u' u₀ u₁ u₂
+
+variables {α : Sort u₀}
+variables {β : Sort u₁}
+variables {γ : Sort u₂}
+variables {σ : Sort u'}
+
+structure var (α : Sort u₀) (β : Sort u₁) : Sort (max u₀ u₁+1) :=
+  (apply : α → β)
+
+@[reducible]
+def pred' (α : Sort u) : Type (max u 1) :=
+var.{u 1} α Prop
+
+def pred'.mk := @var.mk
+
+notation x ` ⊨ `:53 y:52 := @var.apply _ _ y x
+
+structure judgement (h y : pred' α) : Prop :=
+(apply : ∀ σ, σ ⊨ h → σ ⊨ y)
+
+infix ` ⊢ `:53 := judgement
+
+def lifted₀ (p : Prop) : pred' α := ⟨ λ _, p ⟩
+def lifted₁ (op : Prop → Prop) (p : pred' α) : pred' α :=
+⟨ λ i, op (i ⊨ p) ⟩
+def lifted₂ (op : Prop → Prop → Prop) (p q : pred' α) : pred' α :=
+⟨ λ i, op (i ⊨ p) (i ⊨ q) ⟩
+
+attribute [simp, predicate] lifted₀ lifted₁ lifted₂
+attribute [predicate] var.apply var.mk pred'.mk
+
+-- def ew (p : pred' α) : Prop :=
+-- ∀ i, i ⊨ p
+@[predicate]
+def False {α} : pred' α := lifted₀ false
+@[predicate]
+def True {α} : pred' α := lifted₀ true
+@[reducible]
+def holds (x : pred' α) := ∀ Γ, judgement Γ x
+
+prefix `⊩ `:53  := holds
+
+def p_or (p₀ p₁ : pred' α) : pred' α :=
+lifted₂ or p₀ p₁
+
+@[simp, predicate]
+lemma p_or_to_fun (p₀ p₁ : pred' α) (x : α)
+: x ⊨ p_or p₀ p₁ ↔ x ⊨ p₀ ∨ x ⊨ p₁ := by refl
+
+def p_and (p₀ p₁ : pred' α) : pred' α :=
+lifted₂ and p₀ p₁
+
+def p_impl (p₀ p₁ : pred' α) : pred' α :=
+lifted₂ implies p₀ p₁
+
+def p_equiv (p₀ p₁ : pred' α) : pred' α :=
+lifted₂ (↔) p₀ p₁
+
+def p_entails (p₀ p₁ : pred' α) : Prop :=
+⊩ p_impl p₀ p₁
+
+def p_not (p : pred' α) : pred' α :=
+lifted₁ not p
+
+def pred.p_exists {β : Sort u'} {t : Sort u} (P : t → pred' β) : pred' β :=
+⟨λ x, ∃ y, x ⊨ P y⟩
+
+class has_p_exists (α : Sort u) (β : Sort u') :=
+  (p_exists : (β → α) → α)
+
+instance pred_has_p_exists {α : Sort u} {β : Sort u'} : has_p_exists (pred' α) β :=
+⟨ @pred.p_exists _ _ ⟩
+
+export has_p_exists (p_exists)
+
+def p_forall {t : Sort u} {β : Sort u'} (P : t → pred' β) : pred' β :=
+⟨ λ x, ∀ y, x ⊨ P y ⟩
+
+notation `∃∃` binders `, ` r:(scoped P, p_exists P) := r
+notation `∀∀` binders `, ` r:(scoped P, p_forall P) := r
+
+infixl ` ⋁ `:65 := p_or
+infixl ` ⋀ `:70 := p_and
+infixr ` ⟶ `:60 := p_impl
+precedence ≡:55
+infixr ` ≡ ` := p_equiv
+infix ` ⟹ `:60 := p_entails
+-- notation `⦃ `:max act ` ⦄`:0 := ew act
+-- Γ ⊢ p
+-- ∀ σ, σ ⊨ Γ → σ ⊨ p
+instance : has_neg (pred' α) := has_neg.mk p_not
+
+def ctx_impl (Γ p q : pred' α) : Prop :=
+Γ ⊢ p ⟶ q
+
+instance {γ : Type _} : has_map (var γ) :=
+{ map := λ α β f x, ⟨ λ y, f $ x.apply y ⟩ }
+instance {γ : Type _} : has_seq (var γ) :=
+{ seq := λ α β f x, ⟨ λ s, f.apply s (x.apply s) ⟩ }
+instance {γ : Type _} : has_pure (var γ) :=
+{ pure := λ α x, ⟨ λ _, x ⟩ }
+
+def v_eq : var α β → var α β → pred' α
+ | ⟨v₀⟩ ⟨v₁⟩ := ⟨λ s, v₀ s = v₁ s⟩
+
+def v_lt {β : Type _} [has_lt β] : var α β → var α β → pred' α
+ | ⟨v₀⟩ ⟨v₁⟩ := ⟨λ s, v₀ s < v₁ s⟩
+
+def v_wf_r [has_well_founded β] : var α β → var α β → pred' α
+ | ⟨v₀⟩ ⟨v₁⟩ := ⟨λ s, has_well_founded.r (v₀ s) (v₁ s)⟩
+
+def v_le {β : Type _} [has_le β] : var α β → var α β → pred' α
+ | ⟨v₀⟩ ⟨v₁⟩ := ⟨λ s, v₀ s ≤ v₁ s⟩
+
+def v_mem {β : Type _} {γ : Type _} [has_mem β γ] : var α β → var α γ → pred' α
+ | ⟨v₀⟩ ⟨v₁⟩ := ⟨λ s, v₀ s ∈ v₁ s⟩
+
+infix ` ≃ `:75 := v_eq
+infix ` ∊ `:75 := v_mem
+infix ` ≺ `:75 := v_lt
+infix ` ≼ `:75 := v_le
+infix ` ≺≺ `:75 := v_wf_r
+infix ` << `:50 := has_well_founded.r
+
+instance val_to_var_coe : has_coe β (var α β) :=
+{ coe := λ x, ⟨ λ _, x ⟩ }
+instance fun_to_var_coe : has_coe (α → β) (var α β) :=
+{ coe := λ f, ⟨ f ⟩ }
+instance var_coe_to_fun : has_coe_to_fun (var σ $ α → β) :=
+{ F := λ _, var σ α → var σ β
+, coe := λ f x, ⟨ λ s, f.apply s $ x.apply s ⟩ }
+
+def proj : var β γ → var α β → var α γ
+ | ⟨p⟩ ⟨f⟩ := ⟨p∘f⟩
+
+infix ` ∘' ` := proj
+
+@[simp, predicate, reducible]
+def contramap (p : pred' α) (f : β → α) : pred' β :=
+p ∘' ↑f
+
+infixr ` '∘ `:90 := contramap
+
+end predicate
